more whitespace tuning

Weidenbach_Book/Propo_CDCL_Termination.thy
@@ -2,12 +2,15 @@ theory Propo_CDCL_Termination
 imports Propo_CDCL
 begin
 
-text \<open>The condition that no learned clause is a tautology is overkill (in the sense that the no-duplicate condition is enough), but we can reuse @{term build_all_simple_clss}.\<close>
+text \<open>The condition that no learned clause is a tautology is overkill (in the sense that the
+  no-duplicate condition is enough), but we can reuse @{term build_all_simple_clss}.\<close>
 definition cdcl_all_inv_mes where
   "cdcl_all_inv_mes S =
     (no_strange_atm S \<and> cdcl_M_level_inv S \<and>  finite (atms_of_m (clauses S))
     \<and>  finite (learned_clauses S) \<and>  (\<forall>s \<in> learned_clauses S. \<not>tautology s)
-    \<and>  distinct_cdcl_state S \<and> cdcl_conflicting S \<and> all_decomposition_implies (clauses S) (get_all_marked_decomposition (trail S)) \<and> cdcl_learned_clause S)"
+    \<and>  distinct_cdcl_state S \<and> cdcl_conflicting S
+    \<and> all_decomposition_implies (clauses S) (get_all_marked_decomposition (trail S))
+    \<and> cdcl_learned_clause S)"
 
 lemma cdcl_all_inv_mes_inv:
   assumes "cdcl S S'" and "cdcl_all_inv_mes S"
@@ -190,7 +193,8 @@ proof (induct rule: cdcl_s.induct)
     unfolding full_def rtranclp_unfold by blast
   thus ?case by fast
 next
-  case (other' S T U) note o =this(1) and ns = this(2,3) and st = this(4) and no_dup = this(5) and S' = this(6) and S = this(7)
+  case (other' S T U) note o =this(1) and ns = this(2,3) and st = this(4) and no_dup = this(5) and
+    S' = this(6) and S = this(7)
   have "Marked L i \<in> set (trail U)" and "Marked L i \<notin> set (trail S)"
     using no_dup unfolding S S' by (auto simp add: rev_image_eqI)
   hence "Marked L i \<in> set (trail T)"
@@ -230,7 +234,8 @@ proof (induct arbitrary: M H M' i rule: rtranclp.induct)
   case (rtrancl_refl a)
   thus ?case by auto
 next
-  case (rtrancl_into_rtrancl S T U) note st = this(1) and IH = this(2) and s = this(3) and U = this(4) and S = this(5) and lev = this(6)
+  case (rtrancl_into_rtrancl S T U) note st = this(1) and IH = this(2) and s = this(3) and
+    U = this(4) and S = this(5) and lev = this(6)
   show ?case
     proof (cases "\<exists>M'. trail T = M' @ Marked L i # H @ M")
       case False
@@ -246,11 +251,13 @@ next
             using arg_cong[OF MV, of "takeWhile (Not o is_marked)"] nmarked
             by (simp add: takeWhile_tail)
           from arg_cong[OF this, of length] have "length M\<^sub>0 \<le> length M'"
-            unfolding length_append by (metis (no_types, lifting) Nat.le_trans le_add1 length_takeWhile_le)
+            unfolding length_append by (metis (no_types, lifting) Nat.le_trans le_add1
+              length_takeWhile_le)
           hence False using nd V by (cases V) auto
           thus ?case by fast
         next
-          case (other' S' T U) note o = this(1) and ns =this(2,3) and cp = this(4) and nd = this(5) and U = this(6) and st = this(7)
+          case (other' S' T U) note o = this(1) and ns =this(2,3) and cp = this(4) and nd = this(5)
+            and U = this(6) and st = this(7)
           obtain M\<^sub>0 where "trail U = M\<^sub>0 @ trail T" and nmarked: "\<forall>l\<in>set M\<^sub>0. \<not> is_marked l"
             using rtranclp_cdcl_cp_dropWhile_trail cp unfolding full0_def by blast
           hence MV: "M' @ Marked L i # H @ M = M\<^sub>0 @ trail T" unfolding U by simp
@@ -282,10 +289,14 @@ next
           hence 5: "trail T = Marked L i # H @ M"and 6: "trail S' = H @ M"
             proof -
               show "trail S' = H @ M"
-                by (metis (no_types) `trail T = Marked L i # trail S'` `trail T = drop (length M\<^sub>0) M' @ Marked L i # H @ M` append_Nil list.sel(3) nd tl_append2)
+                by (metis (no_types) `trail T = Marked L i # trail S'`
+                  `trail T = drop (length M\<^sub>0) M' @ Marked L i # H @ M` append_Nil list.sel(3) nd
+                  tl_append2)
             next
               show "trail T = Marked L i # H @ M"
-                using append.simps(1) list.sel(3) local.other'(5) tl_append2 by (metis (no_types) `trail T = Marked L i # trail S'` `trail T = drop (length M\<^sub>0) M' @ Marked L i # H @ M` )
+                using append.simps(1) list.sel(3) local.other'(5) tl_append2
+                by (metis (no_types) `trail T = Marked L i # trail S'`
+                  `trail T = drop (length M\<^sub>0) M' @ Marked L i # H @ M` )
             qed
           have 7: "cdcl_s\<^sup>*\<^sup>* S' U" using other'.prems(4) st by auto
           have 8: "cdcl_s S' U" "cdcl_s\<^sup>*\<^sup>* U U"
@@ -339,7 +350,8 @@ lemma rtranclp_cdcl_new_marked_at_beginning_is_decided':
   "trail U = M' @ Marked L i # H @ M" and
   "trail R = M" and
   "cdcl_M_level_inv R"
-  shows "\<exists>y y'. cdcl_s\<^sup>*\<^sup>* R y \<and> cdcl_s y y' \<and> \<not> (\<exists>c. trail y = c @ Marked L i # H @ M) \<and> (\<lambda>a b. cdcl_s a b \<and> (\<exists>c. trail a = c @ Marked L i # H @ M))\<^sup>*\<^sup>* y' U"
+  shows "\<exists>y y'. cdcl_s\<^sup>*\<^sup>* R y \<and> cdcl_s y y' \<and> \<not> (\<exists>c. trail y = c @ Marked L i # H @ M)
+    \<and> (\<lambda>a b. cdcl_s a b \<and> (\<exists>c. trail a = c @ Marked L i # H @ M))\<^sup>*\<^sup>* y' U"
 proof -
   fix T'
   obtain S' T T' where
@@ -399,7 +411,8 @@ next
         by fast
       thus ?case by fast
     next
-      case (other' S T U') note o = this(1) and ns = this(2,3) and cp = this(4) and nd = this(5) and trU' = this(6)
+      case (other' S T U') note o = this(1) and ns = this(2,3) and cp = this(4) and nd = this(5)
+        and trU' = this(6)
       have "cdcl_cp\<^sup>*\<^sup>* T U'" using cp unfolding full0_def by blast
       from rtranclp_cdcl_cp_dropWhile_trail[OF this]
       have "\<exists>M'. trail T = M' @ Marked L i # H @ M"
@@ -412,7 +425,8 @@ next
           case (decided X Y) note dec = this(1) and cp = this(3) and ns = this(4,5)
           show ?case using dec cp ns by blast
         next
-          case (backtrack S T) note bt = this(1) and nd = this(2) and cp = this(3) and trT = this(6) and ns = this(4,5)
+          case (backtrack S T) note bt = this(1) and nd = this(2) and cp = this(3) and
+            trT = this(6) and ns = this(4,5)
           obtain MS N U D LS K MS1 MS2 j where
             S: "S = (MS, N, U, get_maximum_level (D + {#LS#}) MS, C_Clause (D + {#LS#}))" and
             T: "T = (Propagated LS (D + {#LS#}) # MS1, N, insert (D + {#LS#}) U,
@@ -450,7 +464,8 @@ lemma cdcl_o_cannot_learn:
   shows "D + {#L#} \<notin> learned_clauses z"
   using assms(1-4,7,8)
 proof (induction rule: cdcl_o_induct)
-  case (backtrack M N U k D' L' K j M1 M2) note decomp = this(1) and levD = this(4) and lev =this(5) and trM = this(6) and DL = this(7) and learned = this(8) and z = this(9)
+  case (backtrack M N U k D' L' K j M1 M2) note decomp = this(1) and levD = this(4) and lev =this(5)
+    and trM = this(6) and DL = this(7) and learned = this(8) and z = this(9)
   obtain M3 where M3: "M = M3 @ M2 @ Marked K (j + 1) # M1"
     using decomp get_all_marked_decomposition_exists_prepend by metis
   have M: "M = c @ Marked Kh i # H" using trM by simp
@@ -464,7 +479,8 @@ proof (induction rule: cdcl_o_induct)
   hence "i > 0" unfolding H[unfolded M3 d] by auto
   show ?case
     proof
-      assume "D + {#L#} \<in> learned_clauses (Propagated L' (D' + {#L'#}) # M1, N, U \<union> {D' + {#L'#}}, j, C_True)"
+      assume "D + {#L#} \<in>
+                learned_clauses (Propagated L' (D' + {#L'#}) # M1, N, U \<union> {D' + {#L'#}}, j, C_True)"
       hence DLD': "D + {#L#} = D' + {#L'#}" using DL by auto
       have L_cKh: "atm_of L \<in> atm_of `lits_of (c @ [Marked Kh i])"
         using LH learned unfolding M DLD'[symmetric] by (fastforce simp add: image_iff)
@@ -475,7 +491,8 @@ proof (induction rule: cdcl_o_induct)
       have DD'[simp]: "D = D'"
         proof (rule ccontr)
           assume "D \<noteq> D'"
-          hence "L' \<in>#  D" using DLD' by (metis add.left_neutral count_single count_union diff_union_cancelR neq0_conv union_single_eq_member)
+          hence "L' \<in>#  D" using DLD' by (metis add.left_neutral count_single count_union
+            diff_union_cancelR neq0_conv union_single_eq_member)
           hence "get_level L' M \<le> get_maximum_level D M"
             using get_maximum_level_ge_get_level by blast
           moreover {
@@ -494,18 +511,22 @@ proof (induction rule: cdcl_o_induct)
                 get_maximum_possible_level_ge_get_maximum_level) }
           moreover
             have "L \<in># D'"
-              by (metis DLD' `D \<noteq> D'` add.left_neutral count_single count_union diff_union_cancelR neq0_conv union_single_eq_member)
+              by (metis DLD' `D \<noteq> D'` add.left_neutral count_single count_union diff_union_cancelR
+                neq0_conv union_single_eq_member)
             hence "get_maximum_level D' M \<ge> get_level L M"
               using get_maximum_level_ge_get_level by blast
           moreover {
             have "get_all_levels_of_marked (c @ [Marked Kh i]) = rev [i..< k+1]"
-              using append_cons_eq_upt_length_i_end[of " rev (get_all_levels_of_marked H)" i "rev (get_all_levels_of_marked c)" "Suc 0" "Suc k"] H
+              using append_cons_eq_upt_length_i_end[of " rev (get_all_levels_of_marked H)" i
+                "rev (get_all_levels_of_marked c)" "Suc 0" "Suc k"] H
               unfolding M apply (auto simp add: rev_swap[symmetric])
-                by (metis (no_types, hide_lams) Nil_is_append_conv Suc_le_eq less_Suc_eq list.sel(1) rev.simps(2) rev_rev_ident upt_Suc upt_rec)
+                by (metis (no_types, hide_lams) Nil_is_append_conv Suc_le_eq less_Suc_eq list.sel(1)
+                  rev.simps(2) rev_rev_ident upt_Suc upt_rec)
             have "get_level L M  = get_level L (c @ [Marked Kh i])"
               using L_cKh LH unfolding M lits_of_def by simp
             have "get_level L (c @ [Marked Kh i]) \<ge> i"
-              using L_cKh `get_all_levels_of_marked (c @ [Marked Kh i]) = rev [i..<k + 1]` backtrack.hyps(2) calculation(1,2) by auto
+              using L_cKh `get_all_levels_of_marked (c @ [Marked Kh i]) = rev [i..<k + 1]`
+              backtrack.hyps(2) calculation(1,2) by auto
             hence "get_level L M \<ge> i"
               using M `get_level L M = get_level L (c @ [Marked Kh i])` by auto }
           moreover have "get_maximum_level D' M < get_level L' M"
@@ -599,11 +620,13 @@ proof (induction rule: rtranclp.induct)
   case rtrancl_refl
   thus ?case by auto[1]
 next
-  case (rtrancl_into_rtrancl S T U) note st = this(1) and s = this(2) and IH = this(3)[OF this(4-6)] and lev = this(4) and trS = this(5) and DL_S = this(6) and trU = this(7)
+  case (rtrancl_into_rtrancl S T U) note st = this(1) and s = this(2) and IH = this(3)[OF this(4-6)]
+    and lev = this(4) and trS = this(5) and DL_S = this(6) and trU = this(7)
   obtain c where c: "trail T = c @ Marked K i # H" using s by auto
   obtain c' where c': "trail U = c' @ Marked K i # H" using trU by blast
   have lev': "cdcl_all_inv_mes T"
-    by (metis (no_types, lifting) lev mono_rtranclp rtranclp_cdcl_all_inv_mes_inv rtranclp_cdcl_s_rtranclp_cdcl st)
+    by (metis (no_types, lifting) lev mono_rtranclp rtranclp_cdcl_all_inv_mes_inv
+      rtranclp_cdcl_s_rtranclp_cdcl st)
   hence confl': "\<forall>Ta. conflicting T = C_Clause Ta \<longrightarrow> trail T \<Turnstile>as CNot Ta"
     unfolding cdcl_all_inv_mes_def cdcl_learned_clause_def by blast
   show ?case
@@ -641,15 +664,18 @@ lemma no_relearned_clause:
 proof -
   obtain M N U k D L i M1 M2_loc K where
     S: "S = (M, N, U, k, C_Clause (D + {#L#}))"  and
-    T: "T = (Propagated L (D + {#L#}) # M1, N, insert (D + {#L#}) U, get_maximum_level D M, C_True)" and
-    decomp: "(Marked K (Suc (get_maximum_level D M)) # M1, M2_loc) \<in> set (get_all_marked_decomposition M)" and
+    T: "T = (Propagated L (D + {#L#}) # M1, N, insert (D + {#L#}) U, get_maximum_level D M, C_True)"
+      and
+    decomp: "(Marked K (Suc (get_maximum_level D M)) # M1, M2_loc) \<in>
+                set (get_all_marked_decomposition M)" and
     k: "get_level L M = k" and
     level: "get_level L M = get_maximum_level (D+{#L#}) M" and
     i: "get_maximum_level D M = i"
     using  backtrackE[OF bt] by metis
   obtain M2 where
     M: "M = M2 @ Marked K (i+1) # M1"
-    using get_all_marked_decomposition_exists_prepend[OF decomp] i by (metis Suc_eq_plus1 append_assoc)
+    using get_all_marked_decomposition_exists_prepend[OF decomp] i
+    by (metis Suc_eq_plus1 append_assoc)
 
   have invS: "cdcl_all_inv_mes S"
     using invR rtranclp_cdcl_all_inv_mes_inv rtranclp_cdcl_s_rtranclp_cdcl st' by blast
@@ -671,7 +697,8 @@ proof -
     using vars_of_D distinct_atms_of_incl_not_in_other[of "M2 @ Marked K (i + 1) # []" M1]
     unfolding M by auto
   have M1_D: "M1 \<Turnstile>as CNot D"
-    using vars_in_M1 true_annots_remove_if_notin_vars[of "M2 @ Marked K (i + 1) # []" M1 "CNot D"] `M \<Turnstile>as CNot D` unfolding M lits_of_def by simp
+    using vars_in_M1 true_annots_remove_if_notin_vars[of "M2 @ Marked K (i + 1) # []" M1 "CNot D"]
+    `M \<Turnstile>as CNot D` unfolding M lits_of_def by simp
 
   have get_lvls_M: "get_all_levels_of_marked M = rev [1..<Suc k]"
     using lev' unfolding S cdcl_M_level_inv_def by auto
@@ -693,11 +720,12 @@ proof -
           simp_all
       moreover have "\<forall>l \<in> set ?Ls. \<not>is_marked l" using set_takeWhileD by force
       moreover
-        have "get_all_levels_of_marked M = Kk # get_all_levels_of_marked(tl (dropWhile (Not \<circ> is_marked) M))"
+        have "get_all_levels_of_marked M
+                = Kk # get_all_levels_of_marked(tl (dropWhile (Not \<circ> is_marked) M))"
           apply (subst MLs, subst Kk)
           using calculation(2) by (auto simp add: get_all_levels_of_marked_no_marked)
         hence "Kk =  k"
-        using calculation(2) unfolding get_lvls_M by (auto split: split_if_asm simp add: upt.simps(2))
+        using calculation(2) by (auto split: split_if_asm simp add: get_lvls_M upt.simps(2))
       moreover have "set M1 \<subseteq> set (tl (dropWhile (Not o is_marked) M))"
         unfolding M by (induction M2) auto
       ultimately show ?thesis using that MLs by metis
@@ -721,7 +749,10 @@ proof -
     RY: "cdcl_s\<^sup>*\<^sup>* R Y" and
     YZ: "cdcl_s Y Z" and
     nt: "\<not> (\<exists>c. trail Y = c @ Marked K k # M1' @ [])" and
-    Z: "(\<lambda>a b. cdcl_s a b \<and> (\<exists>c. trail a = c @ Marked K k # M1' @ []))\<^sup>*\<^sup>* Z (Ls @ Marked K k # M1', N, U, k, C_Clause (D + {#L#}))"
+    Z: "(\<lambda>a b. cdcl_s a b
+      \<and> (\<exists>c. trail a = c @ Marked K k # M1' @ []))\<^sup>*\<^sup>*
+                Z
+                (Ls @ Marked K k # M1', N, U, k, C_Clause (D + {#L#}))"
     using rtranclp_cdcl_new_marked_at_beginning_is_decided'[OF  st' _ _ lev, of Ls K k M1' "[]"]
     unfolding R M' S by auto
 
@@ -736,7 +767,8 @@ proof -
     using cdcl_s_trail_has_new_marked_is_decide_step[OF YZ nt Z] unfolding trail_conv by auto
   have trY: "trail Y = M1'"
     proof -
-      obtain M' where M: "trail Z = M' @ Marked K k # M1'" using rtranclp_cdcl_s_with_trail_end_has_trail_end[OF Z] by auto
+      obtain M' where M: "trail Z = M' @ Marked K k # M1'"
+        using rtranclp_cdcl_s_with_trail_end_has_trail_end[OF Z] by auto
       obtain M'' where M'': "trail Z = M'' @ trail Y'" and "\<forall>m\<in>set M''. \<not>is_marked m"
         using Y'Z rtranclp_cdcl_cp_dropWhile_trail' unfolding full0_def by blast
       obtain M''' where "trail Y' = M''' @ Marked K k # M1'"
@@ -765,11 +797,13 @@ proof -
       using dec Y'Z rtranclp_cdcl_cp_learned_clause_inv[of Y' Z] unfolding full0_def
       by auto
     have invZ: "cdcl_all_inv_mes Z"
-      by (meson RY YZ invR r_into_rtranclp rtranclp_cdcl_all_inv_mes_inv rtranclp_cdcl_s_rtranclp_cdcl)
+      by (meson RY YZ invR r_into_rtranclp rtranclp_cdcl_all_inv_mes_inv
+        rtranclp_cdcl_s_rtranclp_cdcl)
     have "D + {#L#} \<notin> learned_clauses (Ls @ Marked K k # M1', N, U, k, C_Clause (D + {#L#}))"
       apply (rule rtranclp_cdcl_s_with_trail_end_has_not_been_learned[OF Z invZ trZ])
          using DL lY_lZ apply simp
-        apply (metis (no_types, lifting) `set M1 \<subseteq> set M1'` image_mono lits_of_def order_trans vars_of_D)
+        apply (metis (no_types, lifting) `set M1 \<subseteq> set M1'` image_mono lits_of_def order_trans
+          vars_of_D)
        using L_notin `no_dup M` unfolding M' by (auto simp add: image_iff lits_of_def)
     hence False
       using already_learned DL confl rtranclp_cdcl_s_no_more_clauses st'
@@ -781,7 +815,8 @@ qed
 
 subsection \<open>Decrease of a measure\<close>
 fun cdcl_measure where
-"cdcl_measure (M, N, U, k, C_True) = [(3::nat) ^(card (atms_of_m N)) - card U, 1, card (atms_of_m N) - length M]" |
+"cdcl_measure (M, N, U, k, C_True) =
+  [(3::nat) ^(card (atms_of_m N)) - card U, 1, card (atms_of_m N) - length M]" |
 "cdcl_measure (M, N, U, k, _) = [3 ^(card (atms_of_m N)) - card U, 0, length M]"
 
 lemma length_model_le_vars:
@@ -791,7 +826,8 @@ lemma length_model_le_vars:
   shows "length (trail S) \<le> card (atms_of_m (clauses S))"
 proof -
   obtain M N U k D where S: "S = (M, N, U, k, D)" by (case_tac S, auto)
-  have "finite (atm_of ` lits_of (trail S))" using assms(1,3) unfolding S by (auto simp add: finite_subset)
+  have "finite (atm_of ` lits_of (trail S))"
+    using assms(1,3) unfolding S by (auto simp add: finite_subset)
   have "length (trail S) = card (atm_of ` lits_of (trail S))"
     using no_dup_length_eq_card_atm_of_lits_of no_d by blast
   thus ?thesis using assms(1) by (auto simp add: assms(3) card_mono)
@@ -818,7 +854,8 @@ proof -
 qed
 
 lemma lexn3[simp]:
-  "a < a' \<or> (a = a' \<and> b < b') \<or> (a = a' \<and> b = b' \<and> c < c') \<Longrightarrow> ([a::nat, b, c], [a', b', c']) \<in> lexn {(x, y). x < y} 3 "
+  "a < a' \<or> (a = a' \<and> b < b') \<or> (a = a' \<and> b = b' \<and> c < c')
+    \<Longrightarrow> ([a::nat, b, c], [a', b', c']) \<in> lexn {(x, y). x < y} 3 "
   apply auto
   unfolding lexn_conv apply fastforce
   unfolding lexn_conv apply auto
@@ -828,9 +865,11 @@ lemma lexn3[simp]:
 lemma cdcl_measure_decreasing:
   fixes S :: "'v::linorder cdcl_state"
   assumes "cdcl S S'"
-  and "\<not>(learned_clauses S = learned_clauses S' \<and> [] = trail S' \<and> conflicting S' = C_True)" (*no restart*)
+  and "\<not>(learned_clauses S = learned_clauses S' \<and> [] = trail S' \<and> conflicting S' = C_True)"
+    (*no restart*)
   and "learned_clauses S \<subseteq> learned_clauses S'" (*no forget*)
-  and "backtrack S S' \<Longrightarrow> \<forall>T. conflicting S = C_Clause T \<longrightarrow> T \<notin> learned_clauses S" (*replace 2.10.5-8 we will prove later*)
+  and "backtrack S S' \<Longrightarrow> \<forall>T. conflicting S = C_Clause T \<longrightarrow> T \<notin> learned_clauses S"
+    (*replace 2.10.5-8 we will prove later*)
   and "no_strange_atm S"
   and "cdcl_M_level_inv S"
   and "finite (atms_of_m (clauses S))"
@@ -841,10 +880,13 @@ lemma cdcl_measure_decreasing:
   shows "(cdcl_measure S', cdcl_measure S) \<in> lexn {(a, b). a < b} 3"
   using assms
 proof (induct rule: cdcl_all_induct)
-  case (propagate M N U k C L) note alien = this(7) and M_level = this(8) and no_dup = this(12) and confl = this(13)
-  have propa: "propagate (M, N, U, k, C_True) (Propagated L (C + {#L#}) # M, N, U, k, C_True)" using propagate_rule[OF _ propagate.hyps(1,2)] propagate.hyps(3) by auto
+  case (propagate M N U k C L) note alien = this(7) and M_level = this(8) and no_dup = this(12) and
+    confl = this(13)
+  have propa: "propagate (M, N, U, k, C_True) (Propagated L (C + {#L#}) # M, N, U, k, C_True)"
+    using propagate_rule[OF _ propagate.hyps(1,2)] propagate.hyps(3) by auto
   hence no_dup': "no_dup (Propagated L (C + {#L#}) # M)"
-    unfolding cdcl_M_level_inv_def by (metis M_level cdcl.simps cdcl_M_level_inv_decomp(2) cdcl_consistent_inv trail_conv)
+    unfolding cdcl_M_level_inv_def by (metis M_level cdcl.simps cdcl_M_level_inv_decomp(2)
+      cdcl_consistent_inv trail_conv)
 
   have "no_strange_atm (Propagated L (C + {#L#}) # M, N, U, k, C_True)"
     using alien cdcl.propagate cdcl_no_strange_atm_inv propa by blast
@@ -862,9 +904,11 @@ next
       using decided(7) other[OF cdcl_o.decided[OF deciding[OF _ decided.hyps]]] cdcl_consistent_inv
       unfolding cdcl_M_level_inv_def by fast
     have "no_strange_atm (Marked L (k + 1) # M, N, U, k + 1, C_True)"
-      by (meson decided.intros[OF _ decided.hyps(1,2)] cdcl_no_strange_atm_inv cdcl_o.decided other p(2)   cdcl_no_strange_atm_inv cdcl_o.decided other)
+      by (meson decided.intros[OF _ decided.hyps(1,2)] cdcl_no_strange_atm_inv cdcl_o.decided other
+        p(2) cdcl_no_strange_atm_inv cdcl_o.decided other)
     hence "length (Marked L (k + 1) # M) \<le> card (atms_of_m N)"
-      using no_dup decided(8) length_model_le_vars[of "(Marked L (k + 1) # M, N, U, k + 1, C_True)"] by fastforce
+      using no_dup decided(8) length_model_le_vars[of "(Marked L (k + 1) # M, N, U, k + 1, C_True)"]
+      by fastforce
   ultimately show ?case unfolding decided.hyps(1) by force
 next
   case (skip M N L C' D k U) note  p = this(5,6,7)
@@ -889,14 +933,24 @@ next
   have "D + {#L#} \<notin> U"
     using backtrack.prems(3) backtracking[OF _ backtrack.hyps(1-4)] unfolding S by auto
   hence "card (insert (D + {#L#}) U) = Suc (card U)" by (simp add: `finite U`)
-  have "distinct_cdcl_state ?S'" using backtrack.prems(9) cdcl_o.backtrack[OF backtracking[OF _ backtrack.hyps]] distinct_cdcl_state_inv cdcl.other by blast
-  moreover have "\<forall>s\<in>learned_clauses ?S'. \<not> tautology s" using learned_clauses_are_not_tautologies[OF cdcl.other[OF cdcl_o.backtrack[OF backtracking[OF _ backtrack.hyps]]]] backtrack.prems(5,8,10) by auto
+  have "distinct_cdcl_state ?S'"
+    using backtrack.prems(9) cdcl_o.backtrack[OF backtracking[OF _ backtrack.hyps]]
+    distinct_cdcl_state_inv cdcl.other by blast
+  moreover have "\<forall>s\<in>learned_clauses ?S'. \<not> tautology s"
+    using learned_clauses_are_not_tautologies[OF cdcl.other[OF cdcl_o.backtrack[OF
+      backtracking[OF _ backtrack.hyps]]]] backtrack.prems(5,8,10) by auto
   moreover have "finite (learned_clauses ?S')" using `finite U` by auto
-  moreover have "card (atms_of_m (learned_clauses (M, N, U, k, C_Clause (D + {#L#})))) \<le> card (atms_of_m N)" using backtrack.prems(4,6) card_mono[OF backtrack.prems(6)] local.backtrack(1) unfolding no_strange_atm_def by auto
-  ultimately have "card (U \<union> {D + {#L#}}) \<le> 3 ^ card (atms_of_m (U \<union> {D + {#L#}}))" using learned_clauses_less_upper_bound[of ?S'] by auto
+  moreover have "card (atms_of_m (learned_clauses (M, N, U, k, C_Clause (D + {#L#}))))
+    \<le> card (atms_of_m N)"
+    using backtrack.prems(4,6) card_mono[OF backtrack.prems(6)] local.backtrack(1)
+    unfolding no_strange_atm_def by auto
+  ultimately have "card (U \<union> {D + {#L#}}) \<le> 3 ^ card (atms_of_m (U \<union> {D + {#L#}}))"
+    using learned_clauses_less_upper_bound[of ?S'] by auto
   moreover
-    have "atms_of_m (U \<union> {D + {#L#}}) \<subseteq> atms_of_m N" using backtrack.prems(4) local.backtrack(1) unfolding no_strange_atm_def by auto
-    hence "card (atms_of_m (U \<union> {D + {#L#}})) \<le> card (atms_of_m N)" using card_mono backtrack.prems(6) unfolding S by fastforce
+    have "atms_of_m (U \<union> {D + {#L#}}) \<subseteq> atms_of_m N"
+      using backtrack.prems(4) local.backtrack(1) unfolding no_strange_atm_def by auto
+    hence "card (atms_of_m (U \<union> {D + {#L#}})) \<le> card (atms_of_m N)"
+      using card_mono backtrack.prems(6) unfolding S by fastforce
     hence "(3::nat) ^ card (atms_of_m (U \<union> {D + {#L#}})) \<le> 3 ^ card (atms_of_m N)" by simp
   ultimately have "(3::nat) ^ card (atms_of_m N) \<ge> card (U \<union> {D + {#L#}})" using le_trans by blast
   thus ?case using backtrack.prems(3) unfolding S by (auto simp add: `finite U` `D + {#L#} \<notin> U`)
@@ -997,7 +1051,7 @@ proof -
       have "cdcl_all_inv_mes T"
         using cdcl_all_inv_mes_inv other other'.hyps(1) other'.prems(4) by blast
       from tranclp_cdcl_cp_measure_decreasing[OF _ this]
-      have "(cdcl_measure U, cdcl_measure T) \<in> lexn {a. case a of (a, b) \<Rightarrow> a < b} 3 \<or>
+      have le_or_eq: "(cdcl_measure U, cdcl_measure T) \<in> lexn {a. case a of (a, b) \<Rightarrow> a < b} 3 \<or>
         cdcl_measure U = cdcl_measure T"
         using cp unfolding full0_def rtranclp_unfold by blast
       moreover
@@ -1012,7 +1066,8 @@ proof -
           case (resolve)
           thus ?case by auto
         next
-          case (backtrack S T) note bt = this(1) and st = this(2) and R = this(3) and invR = this(4) and inv = this(5)
+          case (backtrack S T) note bt = this(1) and st = this(2) and R = this(3) and invR = this(4)
+            and inv = this(5)
           have no_relearn: "\<forall>T. conflicting S = C_Clause T \<longrightarrow> T \<notin> learned_clauses S"
             using no_relearned_clause[OF invR st bt] R by (meson Un_iff cdcl_all_inv_mes_def invR)
           show ?case
@@ -1023,10 +1078,13 @@ proof -
         qed
       ultimately show ?case
          proof -
-           have "cdcl_measure U = cdcl_measure T \<longrightarrow> (cdcl_measure U, cdcl_measure S) \<in> lexn {p. case p of (n, na) \<Rightarrow> n < na} 3"
-             using `(cdcl_measure T, cdcl_measure S) \<in> lexn {a. case a of (a, b) \<Rightarrow> a < b} 3` by presburger
+           have "cdcl_measure U = cdcl_measure T \<longrightarrow> (cdcl_measure U, cdcl_measure S)
+             \<in> lexn {p. case p of (n, na) \<Rightarrow> n < na} 3"
+             using `(cdcl_measure T, cdcl_measure S) \<in> lexn {a. case a of (a, b) \<Rightarrow> a < b} 3`
+             by presburger
            thus ?thesis
-             using lexn_trans[OF trans_le, of 3] `(cdcl_measure T, cdcl_measure S) \<in> lexn {a. case a of (a, b) \<Rightarrow> a < b} 3` `(cdcl_measure U, cdcl_measure T) \<in> lexn {a. case a of (a, b) \<Rightarrow> a < b} 3 \<or> cdcl_measure U = cdcl_measure T` unfolding trans_def by blast
+             using lexn_trans[OF trans_le, of 3] `(cdcl_measure T, cdcl_measure S)
+               \<in> lexn {a. case a of (a, b) \<Rightarrow> a < b} 3` le_or_eq unfolding trans_def by blast
          qed
     qed
 qed
@@ -1055,25 +1113,30 @@ proof -
   thus ?thesis using pl tranclp_cdcl_s_decreasing by fast
 qed
 
+(* TODO Move *)
 lemma wf_if_measure_f_notation2:
-assumes "wf r"
-shows "wf {(b, h a)|b a. (f b, f (h a)) \<in> r}"
-apply (rule wf_subset)
-using wf_if_measure_f[OF assms, of f] by auto
+  assumes "wf r"
+  shows "wf {(b, h a)|b a. (f b, f (h a)) \<in> r}"
+  apply (rule wf_subset)
+  using wf_if_measure_f[OF assms, of f] by auto
 
 lemma wf_wf_if_measure'_notation2:
 assumes "wf r" and H: "(\<And>x y. P x \<Longrightarrow> g x y \<Longrightarrow> (f y, f (h x)) \<in> r)"
 shows " wf {(y,h x)| y x. P x \<and> g x y}"
 proof -
   have "wf {(b, h a)|b a. (f b, f (h a)) \<in> r}" using assms(1) wf_if_measure_f_notation2 by auto
-  hence "wf {(b, h a)|b a. P a \<and> g a b \<and> (f b, f (h a)) \<in> r}" using wf_subset[of _ "{(b, h a)| b a. P a \<and> g a b \<and> (f b, f (h a)) \<in> r}"] by auto
-  moreover have "{(b, h a)|b a. P a \<and> g a b \<and> (f b, f (h a)) \<in> r} \<subseteq> {(b, h a)|b a. (f b, f (h a)) \<in> r}" by auto
-  moreover have "{(b, h a)|b a. P a \<and> g a b \<and> (f b, f (h a)) \<in> r} = {(b, h a)|b a. P a \<and> g a b}" using H by auto
+  hence "wf {(b, h a)|b a. P a \<and> g a b \<and> (f b, f (h a)) \<in> r}"
+    using wf_subset[of _ "{(b, h a)| b a. P a \<and> g a b \<and> (f b, f (h a)) \<in> r}"] by auto
+  moreover have "{(b, h a)|b a. P a \<and> g a b \<and> (f b, f (h a)) \<in> r}
+    \<subseteq> {(b, h a)|b a. (f b, f (h a)) \<in> r}" by auto
+  moreover have "{(b, h a)|b a. P a \<and> g a b \<and> (f b, f (h a)) \<in> r} = {(b, h a)|b a. P a \<and> g a b}"
+    using H by auto
   ultimately show ?thesis using wf_subset by simp
 qed
 
 lemma tranclp_cdcl_s_wf:
-  "wf {(S::'v::linorder cdcl_state, S0_cdcl N)| S N. (finite (atms_of_m N) \<and> distinct_mset_set N) \<and> cdcl_s\<^sup>+\<^sup>+ (S0_cdcl N) S}"
+  "wf {(S::'v::linorder cdcl_state, S0_cdcl N)| S N. (finite (atms_of_m N) \<and> distinct_mset_set N)
+    \<and> cdcl_s\<^sup>+\<^sup>+ (S0_cdcl N) S}"
   apply (rule wf_wf_if_measure'_notation2[of "lexn {(a, b). a < b} 3" _ _ cdcl_measure])
    apply (simp add: wf wf_lexn)
   using tranclp_cdcl_s_S0_decreasing by blast
@@ -1089,7 +1152,8 @@ lemma "([1, 2, 3], [1,2, 2]) \<in> lenlex ({(b::int, a). b > a})"
   done
 fun trail_mes ::  "'v::linorder cdcl_state \<Rightarrow> nat list" where
 "trail_mes (M, N, U, k, C) =
-  rev (map (\<lambda>(_, propa). latm propa N) (get_all_marked_decomposition M)) @ [card U, if C = C_True then 1 else 0]"
+  rev (map (\<lambda>(_, propa). latm propa N) (get_all_marked_decomposition M))
+    @ [card U, if C = C_True then 1 else 0]"
 
 lemma
   fixes S :: "'v::linorder cdcl_state"
